Update impl, draft wf soundness.

Earley.thy
@@ -1,9 +1,13 @@
 theory Earley
-  imports 
-    LocalLexing.CFG
-    LocalLexing.Derivations
-    LocalLexing.LLEarleyParsing \<comment>\<open>Rewritten\<close>
-    LocalLexing.Validity \<comment>\<open>TODO: Rewrite\<close>
+  imports
+    "HOL-Library.While_Combinator"
+    LocalLexing.ListTools \<comment>\<open>Use\<close>
+    LocalLexing.InductRules \<comment>\<open>Use\<close>
+    LocalLexing.CFG \<comment>\<open>Use\<close>
+    LocalLexing.Derivations \<comment>\<open>Use\<close>
+    LocalLexing.LocalLexing \<comment>\<open>Done\<close>
+    LocalLexing.LLEarleyParsing \<comment>\<open>Done\<close>
+    LocalLexing.Validity \<comment>\<open>Done\<close>
     LocalLexing.TheoremD2 \<comment>\<open>TODO: Rewrite\<close>
     LocalLexing.TheoremD4 \<comment>\<open>TODO: Rewrite\<close>
     LocalLexing.TheoremD5 \<comment>\<open>TODO: Extract relevant lemmas?\<close>
@@ -19,8 +23,6 @@ theory Earley
     LocalLexing.TheoremD14 \<comment>\<open>TODO: Extract relevant lemmas?\<close>
     LocalLexing.PathLemmas \<comment>\<open>TODO: Extract relevant lemmas?\<close>
     LocalLexing.MainTheorems \<comment>\<open>TODO: Extract relevant lemmas?\<close>
-    LocalLexing.InductRules \<comment>\<open>Needed?\<close>
-    LocalLexing.ListTools \<comment>\<open>Needed?\<close>
 begin
 
 section \<open>Auxiliary Lemmas\<close>
@@ -32,6 +34,21 @@ lemma (in CFG) is_sentence_simp:
 lemma (in CFG) is_word_simp:
   "is_word s \<longleftrightarrow> (\<forall>x \<in> set s. is_terminal x)"
   unfolding is_word_def by (simp add: list_all_iff)
+
+section \<open>List Auxiliary\<close>
+
+fun contains :: "('a \<Rightarrow> bool) \<Rightarrow> 'a list \<Rightarrow> bool" where
+  "contains _ [] \<longleftrightarrow> False"
+| "contains f (x#xs) \<longleftrightarrow> (if f x then True else contains f xs)"
+
+fun slice :: "nat \<Rightarrow> nat \<Rightarrow> 'a list \<Rightarrow> 'a list" where
+  "slice _ _ [] = []"
+| "slice _ 0 (x#xs) = []"
+| "slice 0 (Suc b) (x#xs) = x # slice 0 b xs"
+| "slice (Suc a) (Suc b) (x#xs) = slice a b xs"
+
+lemma "slice a b xs = drop a (take b xs)"
+  by (induction a b xs rule: slice.induct) auto
 
 section \<open>Earley Parsing Algorithm\<close>
 
@@ -49,7 +66,7 @@ datatype item =
     (item_dot : nat) 
     (item_origin : nat)
 
-type_synonym items = "item set"
+type_synonym items = "item list"
 
 definition item_rule_head :: "item \<Rightarrow> symbol" where
   "item_rule_head x = rule_head (item_rule x)"
@@ -78,9 +95,20 @@ definition next_symbol :: "item \<Rightarrow> symbol option" where
 definition inc_item :: "item \<Rightarrow> item" where
   "inc_item x = Item (item_rule x) (item_dot x + 1) (item_origin x)"
 
-type_synonym bin = "item list"
+datatype bin =
+  Bin
+    (items: items)
+
+definition bin_size :: "bin \<Rightarrow> nat" where
+  "bin_size b = length (items b)"
+
+definition bin_append :: "bin \<Rightarrow> item list \<Rightarrow> bin" where
+  "bin_append b is = Bin (items b @ (filter (\<lambda>i. \<not> contains (\<lambda>i'. i = i') (items b)) is))"
 
 type_synonym bins = "bin list"
+
+definition bins_append :: "bins \<Rightarrow> nat \<Rightarrow> item list \<Rightarrow> bins" where
+  "bins_append bs k is = bs[k := bin_append (bs!k) is]"
 
 datatype state =
   State
@@ -88,60 +116,58 @@ datatype state =
     (bin: nat) \<comment>\<open>active bin index\<close>
     (index: nat) \<comment>\<open>active item index\<close>
 
-definition is_finished_state :: "state \<Rightarrow> bool" where
-  "is_finished_state s \<longleftrightarrow> bin s \<ge> length (bins s)"
+definition state_is_final :: "state \<Rightarrow> bool" where
+  "state_is_final s \<longleftrightarrow> bin s \<ge> length (bins s)"
 
-definition is_finished_bin :: "state \<Rightarrow> bool" where
-  "is_finished_bin s \<longleftrightarrow> index s \<ge> length ((bins s)!(bin s))"
+definition state_bin_is_finished :: "state \<Rightarrow> bool" where
+  "state_bin_is_finished s \<longleftrightarrow> index s \<ge> bin_size ((bins s)!(bin s))"
 
-definition current_item :: "state \<Rightarrow> item" where
-  "current_item s = ((bins s)!(bin s))!index s"
-
-fun contains :: "('a \<Rightarrow> bool) \<Rightarrow> 'a list \<Rightarrow> bool" where
-  "contains _ [] \<longleftrightarrow> False"
-| "contains f (x#xs) \<longleftrightarrow> (if f x then True else contains f xs)"
-  
-definition update_bins :: "bins \<Rightarrow> nat \<Rightarrow> item list \<Rightarrow> bins" where
-  "update_bins bs k is = (
-    let bin = bs!k in
-    let is = filter (\<lambda>i. \<not> contains (\<lambda>j. i = j) bin) is in
-    (bs[k := bin @ is])
-  )"
+definition state_current_item :: "state \<Rightarrow> item" where
+  "state_current_item s = (items ((bins s)!(bin s)))!index s"
 
 subsection \<open>Earley Algorithm\<close>
 
 locale Earley = CFG +
   fixes doc :: "symbol list"
   fixes rules :: "rule list"
-  assumes valid_doc: "set Doc \<subseteq> \<TT>"
+  assumes valid_doc: "set doc \<subseteq> \<TT>"
   assumes valid_rules: "set rules = \<RR> \<and> distinct rules"
 begin
 
+definition scan :: "symbol \<Rightarrow> item \<Rightarrow> bins \<Rightarrow> nat \<Rightarrow> bins" where
+  "scan x item bs k = (
+    if doc!k = x then
+      let item' = inc_item item in
+      bins_append bs (k+1) [item']
+    else bs)"
+
+definition predict :: "symbol \<Rightarrow> bins \<Rightarrow> nat \<Rightarrow> bins" where
+  "predict X bs k = (
+    let rules' = filter (\<lambda>rule. rule_head rule = X) rules in
+    let items = map (\<lambda>rule. init_item rule k) rules' in
+    bins_append bs k items)"
+
+definition complete :: "item \<Rightarrow> bins \<Rightarrow> nat \<Rightarrow> bins" where
+  "complete item bs k = (
+    let origin_bin = bs!(item_origin item) in
+    let items = filter (\<lambda>item'. next_symbol item' = Some (item_rule_head item)) (items origin_bin) in
+    bins_append bs k (map inc_item items))"
+
 definition earley_step :: "state \<Rightarrow> state" where
   "earley_step s = (
-    if is_finished_state s then
+    if state_is_final s then
       s
-    else if is_finished_bin s then
+    else if state_bin_is_finished s then
       (State (bins s) (bin s + 1) 0)
     else
-      let item = current_item s in
-      case next_symbol item of
-        Some x \<Rightarrow> (
-          if doc!(bin s) = x then \<comment>\<open>Scan: x is a terminal\<close>
-            let item' = inc_item item in
-            State (update_bins (bins s) (bin s + 1) [item']) (bin s) (index s + 1)
-          else \<comment>\<open>Predict: x is a non-terminal\<close>
-            let rules' = filter (\<lambda>rule. rule_head rule = x) rules in
-            let items = map (\<lambda>rule. init_item rule (bin s)) rules' in
-            State (update_bins (bins s) (bin s) items) (bin s) (index s + 1)
-        )
-      | None \<Rightarrow> ( \<comment>\<open>Complete\<close>
-          let origin_bin = (bins s)!(item_origin item) in
-          let items = filter (\<lambda>item'. next_symbol item' = Some (item_rule_head item)) origin_bin in
-          let items' = map inc_item items in
-          State (update_bins (bins s) (bin s) items') (bin s) (index s + 1)
-        )
-  )"
+      let item = state_current_item s in
+      let bins = 
+        case next_symbol item of
+          Some x \<Rightarrow>
+            if is_terminal x then scan x item (bins s) (bin s)
+            else predict x (bins s) (bin s)
+        | None \<Rightarrow> complete item (bins s) (bin s)
+      in State bins (bin s) (index s + 1))"
 
 function earley :: "state \<Rightarrow> state" where \<comment>\<open>TODO: Termination, REMARK: use while combinator\<close>
   "earley s = (
@@ -149,31 +175,33 @@ function earley :: "state \<Rightarrow> state" where \<comment>\<open>TODO: Term
     if (bin s = bin s') \<and> (index s = index s') then
       s
     else
-      earley s'
-  )"
+      earley s')"
   by pat_completeness simp
 termination
   sorry
 
-definition init_earley_state :: "state" where
-  "init_earley_state = (
-    let init_rules = filter (\<lambda>rule. rule_head rule = \<SS>) rules in
-    let init_items = map (\<lambda>rule. init_item rule 0) init_rules in
-    let bins = replicate (length doc + 1) [] in
-    State (update_bins bins 0 init_items) 0 0
-  )"
+definition init_rules :: "rule list" where
+  "init_rules = filter (\<lambda>rule. rule_head rule = \<SS>) rules"
+
+definition init_items :: "item list" where
+  "init_items = map (\<lambda>rule. init_item rule 0) init_rules"
+
+definition init_bins :: "bins" where
+  "init_bins = bins_append (replicate (length doc + 1) (Bin [])) 0 init_items"
+
+definition init_state :: "state" where
+  "init_state = State init_bins 0 0"
 
 definition earley_recognised :: "bool" where
   "earley_recognised \<longleftrightarrow> (
-    let state = earley init_earley_state in
-    contains is_finished ((bins state)!length doc)
-  )"
+    let state = earley init_state in
+    contains is_finished (items ((bins state)!length doc)))"
 
-subsection \<open>Proofs\<close>
+subsection \<open>Termination\<close>
 
 lemma earley_step_fixpoint':
   "earley_step (earley_step s) = s \<Longrightarrow> earley_step s = s"
-  unfolding earley_step_def is_finished_state_def
+  unfolding earley_step_def state_is_final_def
   apply (auto simp: Let_def split!: option.splits if_splits)
   apply (metis Suc_n_not_le_n n_not_Suc_n nat_le_linear le_SucI le_refl state.sel(2,3))+
   done
@@ -181,6 +209,60 @@ lemma earley_step_fixpoint':
 lemma earley_step_fixpoint:
   "(earley_step s = s) \<longleftrightarrow> earley_step (earley_step s) = s"
   using earley_step_fixpoint' by auto
+
+subsection \<open>Wellformedness\<close>
+
+definition wf_item :: "item \<Rightarrow> bool" where 
+  "wf_item item = (
+    item_rule item \<in> \<RR> \<and>
+    item_origin item \<le> length doc \<and>
+    item_dot item \<le> length (item_rule_body item))"
+
+lemma wf_init_items:
+  "\<forall>x \<in> set init_items. wf_item x"
+  by (auto simp: init_items_def init_rules_def valid_rules init_item_def wf_item_def)
+
+lemma is_word_subset: "is_word x \<Longrightarrow> set y \<subseteq> set x \<Longrightarrow> is_word y"
+  by (metis (mono_tags, hide_lams) in_set_conv_nth is_word_def list_all_length subsetCE)
+
+definition wf_bin :: "nat \<Rightarrow> bin \<Rightarrow> bool" where
+  "wf_bin k b \<longleftrightarrow>
+    distinct (items b) \<and>
+    (\<forall>x \<in> set (items b). wf_item x \<and> item_origin x \<le> k)"
+
+definition wf_bins :: "bins \<Rightarrow> bool" where
+  "wf_bins bs \<longleftrightarrow>
+    length bs = length doc \<and>
+    (\<forall>k < length bs. wf_bin k (bs!k))"
+
+lemma wf_init_bins: \<comment>\<open>TODO\<close>
+  "wf_bins init_bins"
+  sorry
+
+definition wf_state :: "state \<Rightarrow> bool" where
+  "wf_state s \<longleftrightarrow>
+    wf_bins (bins s) \<and>
+    (bin s) \<le> length doc \<and>
+    (index s) \<le> bin_size ((bins s)!(bin s))"
+
+lemma wf_init_state: \<comment>\<open>TODO\<close>
+  "wf_state init_state"
+  sorry
+
+subsection \<open>Soundness\<close>
+
+(* off by one ;) *)
+definition sound_item :: "nat \<Rightarrow> item \<Rightarrow> bool" where
+  "sound_item k item = derives [item_rule_head item] (slice (item_origin item) k doc @ item_\<beta> item)"
+
+definition sound_bin :: "nat \<Rightarrow> bin \<Rightarrow> bool" where
+  "sound_bin k b = (\<forall>item \<in> set (items b). sound_item k item)"
+
+definition sound_bins :: "bins \<Rightarrow> bool" where
+  "sound_bins bs = (\<forall>k < length bs. sound_bin k (bs!k))"
+
+definition sound_state :: "state \<Rightarrow> bool" where
+  "sound_state s = sound_bins (bins s)"
 
 end
 
